theories/L6_PCPS/Heap/closure_conversion_util.v
@@ -4,7 +4,7 @@
 
 From L6 Require Import cps cps_util set_util hoisting identifiers ctx
                        Ensembles_util List_util functions eval.
-From L6.Heap Require Import closure_conversion size_cps heap.
+From L6.Heap Require Import closure_conversion compat heap.
 
 Require Import compcert.lib.Coqlib.
 Require Import Coq.ZArith.Znumtheory ArithRing Coq.Relations.Relations Coq.Arith.Wf_nat.
@@ -23,11 +23,10 @@ Close Scope Z_scope.
 
 Module CCUtil (H : Heap).
 
-  Module Size := Size H.
-  
-  Import H Size.C.LR.Sem.Equiv Size.C.LR.Sem.Equiv.Defs Size.C.LR.Sem
-         Size.C.LR Size.C Size.
+  Module C := Compat H.
 
+  Import H C C.LR C.LR.Sem C.LR.Sem.Equiv C.LR.Sem.Equiv.Defs.
+  
   Variable clo_tag : cTag.
 
   (** ** Proof that after closure conversion all functions are closed *)
@@ -586,9 +585,9 @@ Module CCUtil (H : Heap).
   Qed.
 
 
-    Lemma project_var_get Scope Funs c Γ FVs S1 x x' C1 S2 rho1 H1 rho2 H2 m y:
+  Lemma project_var_get Scope Funs c Γ FVs S1 x x' C1 S2 rho1 H1 rho2 H2 m y:
     project_var Scope Funs c Γ FVs S1 x x' C1 S2 ->
-    ctx_to_heap_env C1 H1 rho1 H2 rho2 m ->
+    ctx_to_heap_env_CC C1 H1 rho1 H2 rho2 m ->
     ~ In _ S1 y ->
     M.get y rho1 = M.get y rho2. 
   Proof.
@@ -603,7 +602,7 @@ Module CCUtil (H : Heap).
   
   Lemma project_vars_get Scope Funs c Γ FVs S1 xs xs' C1 S2 rho1 H1 rho2 H2 m y:
     project_vars Scope Funs c Γ FVs S1 xs xs' C1 S2 ->
-    ctx_to_heap_env C1 H1 rho1 H2 rho2 m ->
+    ctx_to_heap_env_CC C1 H1 rho1 H2 rho2 m ->
     ~ In _ S1 y ->
     M.get y rho1 = M.get y rho2. 
   Proof.
@@ -611,7 +610,7 @@ Module CCUtil (H : Heap).
     induction xs; intros Scope Funs Γ FVs S1 xs' C1 S2 rho1 H1 rho2 H2 m y Hproj Hctx Hnin.
     - inv Hproj. inv Hctx. reflexivity.
     - inv Hproj.  
-      edestruct ctx_to_heap_env_comp_ctx_f_l as [rho'' [H'' [m1 [m2  [Hctx1 [Hctx2 Hadd]]]]]]; eauto.
+      edestruct ctx_to_heap_env_CC_comp_ctx_f_l as [rho'' [H'' [m1 [m2  [Hctx1 [Hctx2 Hadd]]]]]]; eauto.
       subst. eapply project_var_get in Hctx1; eauto.
       eapply IHxs in Hctx2; eauto.
       rewrite Hctx1, <- Hctx2. reflexivity.
@@ -621,7 +620,7 @@ Module CCUtil (H : Heap).
   
   Lemma project_var_getlist Scope Funs c Γ FVs S1 x x' C1 S2 rho1 H1 rho2 H2 m ys :
     project_var Scope Funs c Γ FVs S1 x x' C1 S2 ->
-    ctx_to_heap_env C1 H1 rho1 H2 rho2 m ->
+    ctx_to_heap_env_CC C1 H1 rho1 H2 rho2 m ->
     Disjoint _ S1 (FromList ys) ->
     getlist ys rho1 = getlist ys rho2. 
   Proof.
@@ -638,7 +637,7 @@ Module CCUtil (H : Heap).
 
   Lemma project_vars_getlist Scope Funs c Γ FVs S1 xs xs' C1 S2 rho1 H1 rho2 H2 m ys :
     project_vars Scope Funs c Γ FVs S1 xs xs' C1 S2 ->
-    ctx_to_heap_env C1 H1 rho1 H2 rho2 m ->
+    ctx_to_heap_env_CC C1 H1 rho1 H2 rho2 m ->
     Disjoint _ S1 (FromList ys) ->
     getlist ys rho1 = getlist ys rho2. 
   Proof.
@@ -655,7 +654,7 @@ Module CCUtil (H : Heap).
   (** [project_var] preserves env_locs in dom *)
   Lemma project_var_env_locs Scope Funs c Γ FVs x x' C S S' e k rho H rho' H':
     project_var Scope Funs c Γ FVs S x x' C S' ->
-    ctx_to_heap_env C H rho H' rho' k ->
+    ctx_to_heap_env_CC C H rho H' rho' k ->
     well_formed (reach' H (env_locs rho (occurs_free (C |[ e ]|)))) H ->
     env_locs rho (occurs_free (C |[ e ]|)) \subset dom H ->
     env_locs rho' (occurs_free e) \subset dom  H'.
@@ -680,7 +679,7 @@ Module CCUtil (H : Heap).
   
   Lemma project_var_env_locs' Scope Funs c Γ FVs x x' C S S' k rho H rho' H':
     project_var Scope Funs c Γ FVs S x x' C S' ->
-    ctx_to_heap_env C H rho H' rho' k ->
+    ctx_to_heap_env_CC C H rho H' rho' k ->
     well_formed (reach' H (env_locs rho (FV_cc Scope Funs Γ))) H ->
     env_locs rho (FV_cc Scope Funs Γ) \subset dom H ->
     env_locs rho' (x' |: (FV_cc Scope Funs Γ)) \subset dom  H'.
@@ -716,7 +715,7 @@ Module CCUtil (H : Heap).
   (** [project_var] preserves well-formedness *)
   Lemma project_var_well_formed Scope Funs c Γ FVs x x' C S S' e k rho H rho' H':
     project_var Scope Funs c Γ FVs S x x' C S' ->
-    ctx_to_heap_env C H rho H' rho' k ->
+    ctx_to_heap_env_CC C H rho H' rho' k ->
     (env_locs rho (occurs_free (C |[ e ]|))) \subset dom H ->
     well_formed (reach' H (env_locs rho (occurs_free (C |[ e ]|)))) H ->
     well_formed (reach' H' (env_locs rho' (occurs_free e))) H'.
@@ -743,7 +742,7 @@ Module CCUtil (H : Heap).
   
   Lemma project_var_reachable Scope Funs c Γ FVs x x' C S S' e k rho H rho' H':
     project_var Scope Funs c Γ FVs S x x' C S' ->
-    ctx_to_heap_env C H rho H' rho' k ->
+    ctx_to_heap_env_CC C H rho H' rho' k ->
     reach' H' (env_locs rho' (occurs_free e)) \subset
     reach' H (env_locs rho (occurs_free (C |[ e ]|))).
   Proof with (now eauto with Ensembles_DB). 
@@ -763,14 +762,14 @@ Module CCUtil (H : Heap).
   
   Lemma project_vars_reachable Scope Funs c Γ FVs xs xs' C S S' e k rho H rho' H':
     project_vars Scope Funs c Γ FVs S xs xs' C S' ->
-    ctx_to_heap_env C H rho H' rho' k ->
+    ctx_to_heap_env_CC C H rho H' rho' k ->
     reach' H' (env_locs rho' (occurs_free e)) \subset
     reach' H (env_locs rho (occurs_free (C |[ e ]|))).
   Proof with (now eauto with Ensembles_DB).
     intros Hvar. revert rho H rho' H' k e. 
     induction Hvar; intros rho1 H1 rho2 H2 k e Hctx.
     - inv Hctx. reflexivity.
-    - edestruct ctx_to_heap_env_comp_ctx_f_l as [rho3 [H3 [m1 [m2 [Hctx2 [Hctx3 Heq]]]]]].
+    - edestruct ctx_to_heap_env_CC_comp_ctx_f_l as [rho3 [H3 [m1 [m2 [Hctx2 [Hctx3 Heq]]]]]].
       eassumption. subst.
       eapply Included_trans. eapply IHHvar; eauto.
       eapply Included_trans. eapply project_var_reachable; eauto.
@@ -780,7 +779,7 @@ Module CCUtil (H : Heap).
   (** [project_var] preserves well-formedness *)
   Lemma project_var_well_formed' Scope Funs c Γ FVs x x' C S S' k rho H rho' H':
     project_var Scope Funs c Γ FVs S x x' C S' ->
-    ctx_to_heap_env C H rho H' rho' k ->
+    ctx_to_heap_env_CC C H rho H' rho' k ->
     (env_locs rho (FV_cc Scope Funs Γ)) \subset dom H ->
     well_formed (reach' H (env_locs rho (FV_cc Scope Funs Γ))) H ->
     well_formed (reach' H' (env_locs rho' (x' |: (FV_cc Scope Funs Γ)))) H'.
@@ -811,7 +810,7 @@ Module CCUtil (H : Heap).
   
   Lemma project_var_env_locs_subset Scope Funs c Γ FVs xs xs' C S S' S1 k rho H rho' H':
     project_var Scope Funs c Γ FVs S xs xs' C S' ->
-    ctx_to_heap_env C H rho H' rho' k ->
+    ctx_to_heap_env_CC C H rho H' rho' k ->
     Disjoint _ S1 S ->
     env_locs rho' S1 <--> env_locs rho S1.
   Proof with (now eauto with Ensembles_DB). 
@@ -822,14 +821,14 @@ Module CCUtil (H : Heap).
   
    Lemma project_vars_env_locs_subset Scope Funs c Γ FVs xs xs' C S S' S1 k rho H rho' H':
     project_vars Scope Funs c Γ FVs S xs xs' C S' ->
-    ctx_to_heap_env C H rho H' rho' k ->
+    ctx_to_heap_env_CC C H rho H' rho' k ->
     Disjoint _ S1 S ->
     env_locs rho' S1 <--> env_locs rho S1.
   Proof with (now eauto with Ensembles_DB). 
     intros Hvar. revert rho H rho' H' k. 
     induction Hvar; intros rho1 H1 rho2 H2 k Hctx Hd.
     - inv Hctx. reflexivity.
-    - edestruct ctx_to_heap_env_comp_ctx_f_l as [rho3 [H3 [m1 [m2 [Hctx2 [Hctx3 Heq]]]]]].
+    - edestruct ctx_to_heap_env_CC_comp_ctx_f_l as [rho3 [H3 [m1 [m2 [Hctx2 [Hctx3 Heq]]]]]].
       eassumption. subst. rewrite IHHvar; eauto.
       rewrite project_var_env_locs_subset; eauto.
       reflexivity. eapply Disjoint_Included_r; try eassumption.
@@ -838,7 +837,7 @@ Module CCUtil (H : Heap).
 
   Lemma project_var_heap Scope Funs c Γ FVs x x' S S' C H rho H' rho' k :
     project_var Scope Funs c Γ FVs S x x' C S' ->
-    ctx_to_heap_env C H rho H' rho' k ->
+    ctx_to_heap_env_CC C H rho H' rho' k ->
     H = H'. 
   Proof.
     intros Hvar Hctx; inv Hvar; inv Hctx; eauto.
@@ -847,13 +846,13 @@ Module CCUtil (H : Heap).
 
   Lemma project_vars_heap Scope Funs c Γ FVs x x' S S' C H rho H' rho' k :
     project_vars Scope Funs c Γ FVs S x x' C S' ->
-    ctx_to_heap_env C H rho H' rho' k ->
+    ctx_to_heap_env_CC C H rho H' rho' k ->
     H = H'. 
   Proof.
     intros Hvar. revert rho H rho' H' k. 
     induction Hvar; intros rho1 H1 rho2 H2 k Hctx.
     - inv Hctx; eauto.
-    - edestruct ctx_to_heap_env_comp_ctx_f_l as [rho3 [H3 [m1 [m2 [Hctx2 [Hctx3 Heq]]]]]].
+    - edestruct ctx_to_heap_env_CC_comp_ctx_f_l as [rho3 [H3 [m1 [m2 [Hctx2 [Hctx3 Heq]]]]]].
       eassumption. subst.
       eapply project_var_heap in Hctx2; eauto.
       subst. eapply IHHvar; eauto.
@@ -861,7 +860,7 @@ Module CCUtil (H : Heap).
 
   Lemma project_vars_env_locs Scope Funs c Γ FVs xs xs' C S S' e k rho H rho' H':
     project_vars Scope Funs c Γ FVs S xs xs' C S' ->
-    ctx_to_heap_env C H rho H' rho' k ->
+    ctx_to_heap_env_CC C H rho H' rho' k ->
     (env_locs rho (occurs_free (C |[ e ]|))) \subset dom H ->
     well_formed (reach' H (env_locs rho (occurs_free (C |[ e ]|)))) H ->
     (env_locs rho' (occurs_free e)) \subset dom H'.
@@ -869,7 +868,7 @@ Module CCUtil (H : Heap).
     intros Hvar. revert rho H rho' H' k e. 
     induction Hvar; intros rho1 H1 rho2 H2 k e Hctx Hlocs Hwf.
     - inv Hctx. simpl in *; eauto.
-    - edestruct ctx_to_heap_env_comp_ctx_f_l as [rho3 [H3 [m1 [m2 [Hctx2 [Hctx3 Heq]]]]]].
+    - edestruct ctx_to_heap_env_CC_comp_ctx_f_l as [rho3 [H3 [m1 [m2 [Hctx2 [Hctx3 Heq]]]]]].
       eassumption. subst.
       rewrite <- app_ctx_f_fuse in *.
       eapply IHHvar; try eassumption.
@@ -879,7 +878,7 @@ Module CCUtil (H : Heap).
     
   Lemma project_vars_env_locs' Scope Funs c Γ FVs xs xs' C S S' k rho H rho' H':
     project_vars Scope Funs c Γ FVs S xs xs' C S' ->
-    ctx_to_heap_env C H rho H' rho' k ->
+    ctx_to_heap_env_CC C H rho H' rho' k ->
     Disjoint _ S (Scope :|: (Funs \\ Scope)) ->
     well_formed (reach' H (env_locs rho (FV_cc Scope Funs Γ))) H ->
     env_locs rho (FV_cc Scope Funs Γ) \subset dom H ->
@@ -888,7 +887,7 @@ Module CCUtil (H : Heap).
     intros Hvar. revert rho H rho' H' k. 
     induction Hvar; intros rho1 H1 rho2 H2 k Hctx Hd Hlocs Hwf.
     - inv Hctx. rewrite FromList_nil, Union_Empty_set_neut_l. simpl in *; eauto.
-    - edestruct ctx_to_heap_env_comp_ctx_f_l as [rho3 [H3 [m1 [m2 [Hctx2 [Hctx3 Heq]]]]]].
+    - edestruct ctx_to_heap_env_CC_comp_ctx_f_l as [rho3 [H3 [m1 [m2 [Hctx2 [Hctx3 Heq]]]]]].
       eassumption. subst.
       rewrite FromList_cons.
       rewrite <- !Union_assoc. rewrite env_locs_Union.
@@ -910,7 +909,7 @@ Module CCUtil (H : Heap).
   
   Lemma project_vars_well_formed Scope Funs c Γ FVs xs xs' C S S' e k rho H rho' H':
     project_vars Scope Funs c Γ FVs S xs xs' C S' ->
-    ctx_to_heap_env C H rho H' rho' k ->
+    ctx_to_heap_env_CC C H rho H' rho' k ->
     (env_locs rho (occurs_free (C |[ e ]|))) \subset dom H ->
     well_formed (reach' H (env_locs rho (occurs_free (C |[ e ]|)))) H ->
     well_formed (reach' H' (env_locs rho' (occurs_free e))) H'.
@@ -918,7 +917,7 @@ Module CCUtil (H : Heap).
     intros Hvar. revert rho H rho' H' k e. 
     induction Hvar; intros rho1 H1 rho2 H2 k e Hctx Hlocs Hwf.
     - inv Hctx. simpl in *; eauto.
-    - edestruct ctx_to_heap_env_comp_ctx_f_l as [rho3 [H3 [m1 [m2 [Hctx2 [Hctx3 Heq]]]]]].
+    - edestruct ctx_to_heap_env_CC_comp_ctx_f_l as [rho3 [H3 [m1 [m2 [Hctx2 [Hctx3 Heq]]]]]].
       eassumption. subst.
       rewrite <- app_ctx_f_fuse in *.
       eapply IHHvar; try eassumption.
@@ -928,7 +927,7 @@ Module CCUtil (H : Heap).
   
   Lemma project_vars_well_formed' Scope Funs c Γ FVs xs xs' C S S' k rho H rho' H':
     project_vars Scope Funs c Γ FVs S xs xs' C S' ->
-    ctx_to_heap_env C H rho H' rho' k ->
+    ctx_to_heap_env_CC C H rho H' rho' k ->
     Disjoint _ S (Scope :|: (Funs \\ Scope)) ->
     (env_locs rho (FV_cc Scope Funs Γ)) \subset dom H ->
     well_formed (reach' H (env_locs rho (FV_cc Scope Funs Γ))) H ->
@@ -938,7 +937,7 @@ Module CCUtil (H : Heap).
     induction Hvar; intros rho1 H1 rho2 H2 k Hctx HD Hlocs Hwf.
     - inv Hctx. simpl in *; eauto.
       rewrite FromList_nil, Union_Empty_set_neut_l. simpl in *; eauto.
-    - edestruct ctx_to_heap_env_comp_ctx_f_l as [rho3 [H3 [m1 [m2 [Hctx2 [Hctx3 Heq]]]]]].
+    - edestruct ctx_to_heap_env_CC_comp_ctx_f_l as [rho3 [H3 [m1 [m2 [Hctx2 [Hctx3 Heq]]]]]].
       eassumption. subst.
       rewrite FromList_cons.
       rewrite <- !Union_assoc. rewrite env_locs_Union, reach'_Union.
